characteristic/cfScript.sml
@@ -776,6 +776,237 @@ val build_cases_def = Define `
      (!s. validate_pat env.c s pat v env.v))`
 
 (*------------------------------------------------------------------*)
+(* Soundness predicate & lemmas *)
+
+(* States that a hoare triple {H} e {Q} is valid in environment [env] *)
+val htriple_valid_def = Define `
+  htriple_valid (p:'ffi ffi_proj) e env H Q =
+    !st h_i h_k.
+      SPLIT (st2heap p st) (h_i, h_k) ==>
+      H h_i ==>
+      ?v st' h_f h_g.
+        SPLIT3 (st2heap p st') (h_f, h_k, h_g) /\
+        evaluate F env st e (st', Rval v) /\
+        Q v h_f`
+
+(* Soundness for relation [R] *)
+val sound_def = Define `
+  sound (p:'ffi ffi_proj) e R =
+    !env H Q.
+      R env H Q ==>
+      htriple_valid p e env H Q`
+
+
+val htriple_valid_normalise = store_thm ("htriple_valid_normalise",
+  ``!e env H Q.
+      htriple_valid (p:'ffi ffi_proj) (normalise e) env H Q <=>
+      htriple_valid (p:'ffi ffi_proj) e env H Q``,
+  fs [htriple_valid_def, evaluate_normalise]
+);
+
+val sound_normalise = store_thm("sound_normalise",
+  ``sound p (normalise e) R <=> sound p e R``,
+  fs [sound_def, htriple_valid_normalise]);
+
+val star_split = Q.prove (
+  `!H1 H2 H3 H4 h1 h2 h3 h4.
+     ((H1 * H2) (h1 UNION h2) ==> (H3 * H4) (h3 UNION h4)) ==>
+     DISJOINT h1 h2 ==> H1 h1 ==> H2 h2 ==>
+     ?u v. H3 u /\ H4 v /\ SPLIT (h3 UNION h4) (u, v)`,
+  fs [STAR_def] \\ rpt strip_tac \\
+  `SPLIT (h1 UNION h2) (h1, h2)` by SPLIT_TAC \\
+  metis_tac []
+)
+
+val sound_local = store_thm ("sound_local",
+  ``!e R. sound (p:'ffi ffi_proj) e R ==> sound (p:'ffi ffi_proj) e (\env. local (R env))``,
+  rpt strip_tac \\ rewrite_tac [sound_def, htriple_valid_def] \\
+  fs [local_def] \\ rpt strip_tac \\
+  res_tac \\ rename1 `(H_i * H_k) h_i` \\ rename1 `R env H_i Q_f` \\
+  rename1 `SEP_IMPPOST (Q_f *+ H_k) (Q *+ H_g)` \\
+  fs [STAR_def] \\ rename1 `H_i h'_i` \\ rename1 `H_k h'_k` \\
+  `SPLIT (st2heap (p:'ffi ffi_proj) st) (h'_i, h_k UNION h'_k)` by SPLIT_TAC \\
+  qpat_x_assum `sound _ _ _` (progress o REWRITE_RULE [sound_def, htriple_valid_def]) \\
+  rename1 `SPLIT3 _ (h'_f, _, h'_g)` \\
+  fs [SEP_IMPPOST_def, STARPOST_def, SEP_IMP_def, STAR_def] \\
+  first_x_assum (qspecl_then [`v`, `h'_f UNION h'_k`] assume_tac) \\
+  `DISJOINT h'_f h'_k` by SPLIT_TAC \\
+  `?h_f h''_g. Q v h_f /\ H_g h''_g /\ SPLIT (h'_f UNION h'_k) (h_f, h''_g)` by
+    metis_tac [star_split] \\
+  Q.LIST_EXISTS_TAC [`v`, `st'`, `h_f`, `h'_g UNION h''_g`] \\ fs [] \\
+  SPLIT_TAC
+)
+
+val sound_false = store_thm ("sound_false",
+  ``!e. sound (p:'ffi ffi_proj) e (\env H Q. F)``,
+  rewrite_tac [sound_def]
+)
+
+val sound_local_false = Q.prove (
+  `!e. sound (p:'ffi ffi_proj) e (\env. local (\H Q. F))`,
+  strip_tac \\ HO_MATCH_MP_TAC sound_local \\ fs [sound_false]
+)
+
+(*------------------------------------------------------------------*)
+(* Lemmas relating [app], and [htriple_valid] (usually on the
+   expression composing the body of the applied function).
+*)
+
+val app_basic_of_htriple_valid = Q.prove (
+  `!clos body x env v H Q.
+    do_opapp [clos; x] = SOME (env, body) ==>
+    htriple_valid (p:'ffi ffi_proj) body env H Q ==>
+    app_basic (p:'ffi ffi_proj) clos x H Q`,
+  fs [app_basic_def, htriple_valid_def] \\ rpt strip_tac \\
+  first_x_assum progress \\ instantiate \\ SPLIT_TAC
+)
+
+val app_of_htriple_valid = Q.prove (
+  `!ns xvs env body H Q.
+     ns <> [] ==>
+     LENGTH ns = LENGTH xvs ==>
+     htriple_valid (p:'ffi ffi_proj) body (extend_env ns xvs env) H Q ==>
+     app (p:'ffi ffi_proj) (naryClosure env ns body) xvs H Q`,
+
+  Induct \\ rpt strip_tac \\ fs [naryClosure_def, LENGTH_CONS] \\ rw [] \\
+  rename1 `extend_env (n::ns) (xv::xvs) _` \\ Cases_on `ns` \\
+  fs [LENGTH_NIL, LENGTH_CONS] \\ rw [] \\
+  rfs [extend_env_def, Once extend_env_v_def, naryFun_def, app_def]
+  THEN1 (irule app_basic_of_htriple_valid \\ fs [extend_env_v_def, do_opapp_def])
+  THEN1 (
+    rename1 `extend_env_v (n'::ns) (xv'::xvs) _` \\
+    fs [app_basic_def] \\ rpt strip_tac \\ fs [do_opapp_def] \\
+    fs [SEP_EXISTS, cond_def, STAR_def, PULL_EXISTS, SPLIT_emp2] \\
+    fs [naryFun_def, naryClosure_def, Once bigStepTheory.evaluate_cases] \\
+    first_assum progress \\ instantiate \\ qexists_tac `{}` \\ SPLIT_TAC
+  )
+)
+
+val app_rec_of_htriple_valid_aux = Q.prove (
+  `!f body params xvs funs naryfuns env H Q fvs.
+     params <> [] ==>
+     LENGTH params = LENGTH xvs ==>
+     naryfuns = letrec_pull_params funs ==>
+     ALL_DISTINCT (MAP (\ (f,_,_). f) naryfuns) ==>
+     find_recfun f naryfuns = SOME (params, body) ==>
+     htriple_valid (p:'ffi ffi_proj) body
+       (extend_env_rec (MAP (\ (f,_,_). f) naryfuns) fvs params xvs env)
+       H Q ==>
+     fvs = MAP (\ (f,_,_). naryRecclosure env naryfuns f) naryfuns ==>
+     app (p:'ffi ffi_proj) (naryRecclosure env naryfuns f) xvs H Q`,
+
+  Cases_on `params` \\ rpt strip_tac \\ rw [] \\
+  fs [LENGTH_CONS] \\ rfs [] \\ qpat_x_assum `xvs = _` (K all_tac) \\
+  rename1 `extend_env_rec _ _ (n::params) (xv::xvs) _` \\
+  Cases_on `params` \\ rfs [LENGTH_NIL, LENGTH_CONS] \\
+  fs [extend_env_rec_def, extend_env_v_rec_def] \\
+  fs [extend_env_def, extend_env_v_def, app_def]
+  THEN1 (
+    irule app_basic_of_htriple_valid \\
+    progress_then (fs o sing) do_opapp_naryRecclosure \\
+    fs [naryFun_def, letrec_pull_params_names, build_rec_env_zip]
+  )
+  THEN1 (
+    rw [] \\ rename1 `extend_env_v (n'::params) (xv'::xvs) _` \\
+    fs [app_basic_def] \\ rpt strip_tac \\
+    progress_then (fs o sing) do_opapp_naryRecclosure \\
+    fs [SEP_EXISTS, cond_def, STAR_def, PULL_EXISTS, SPLIT_emp2] \\
+    rename1 `SPLIT _ (h, i)` \\
+    `SPLIT3 (st2heap (p:'ffi ffi_proj) st) (h, {}, i)` by SPLIT_TAC \\
+    instantiate \\
+    (* fixme *)
+    qexists_tac `naryClosure
+      (env with v := (n,xv)::(ZIP (MAP (\ (f,_,_). f) (letrec_pull_params funs),
+        MAP (\ (f,_,_). naryRecclosure env (letrec_pull_params funs) f)
+            (letrec_pull_params funs)) ++ env.v))
+      (n'::params) body` \\ strip_tac
+    THEN1 (irule app_of_htriple_valid \\ fs [extend_env_def])
+    THEN1 (
+      fs [naryFun_def, naryClosure_def, Once bigStepTheory.evaluate_cases] \\
+      fs [letrec_pull_params_cancel, letrec_pull_params_names] \\
+      fs [build_rec_env_zip]
+    )
+  )
+)
+
+val app_rec_of_htriple_valid = Q.prove (
+  `!f params body funs xvs env H Q.
+     params <> [] ==>
+     LENGTH params = LENGTH xvs ==>
+     ALL_DISTINCT (MAP (\ (f,_,_). f) funs) ==>
+     find_recfun f (letrec_pull_params funs) = SOME (params, body) ==>
+     htriple_valid (p:'ffi ffi_proj) body
+       (extend_env_rec
+          (MAP (\ (f,_,_). f) funs)
+          (MAP (\ (f,_,_). naryRecclosure env (letrec_pull_params funs) f) funs)
+          params xvs env)
+        H Q ==>
+     app (p:'ffi ffi_proj) (naryRecclosure env (letrec_pull_params funs) f) xvs H Q`,
+  rpt strip_tac \\ irule app_rec_of_htriple_valid_aux
+  THEN1 (fs [letrec_pull_params_names])
+  THEN1 (qexists_tac `funs` \\ fs [])
+  THEN1 (instantiate \\ fs [letrec_pull_params_names])
+)
+
+(*------------------------------------------------------------------*)
+(* Lemmas used in the soundness proof of FFI *)
+
+val SPLIT_SING_2 = store_thm("SPLIT_SING_2",
+  ``SPLIT s (x,{y}) <=> (s = y INSERT x) /\ ~(y IN x)``,
+  SPLIT_TAC);
+
+val SUBSET_IN = prove(
+  ``!s t x. s SUBSET t /\ x IN s ==> x IN t``,
+  fs [SUBSET_DEF] \\ metis_tac []);
+
+val SPLIT_FFI_SET_IMP_DISJOINT = store_thm("SPLIT_FFI_SET_IMP_DISJOINT",
+  ``SPLIT (st2heap p st) (c,{FFI_part s u ns}) ==>
+    !s1. ~(FFI_part s1 u ns IN c)``,
+  fs [SPLIT_def] \\ rw [] \\ fs [EXTENSION,st2heap_def,DISJOINT_DEF]
+  \\ CCONTR_TAC \\ fs []
+  \\ `FFI_part s1 u ns IN ffi2heap p st.ffi /\
+      FFI_part s u ns IN ffi2heap p st.ffi` by
+          metis_tac [FFI_part_NOT_IN_store2heap]
+  \\ PairCases_on `p`
+  \\ fs [ffi2heap_def]
+  \\ pop_assum mp_tac \\ IF_CASES_TAC \\ fs []
+  \\ CCONTR_TAC \\ fs []
+  \\ Cases_on `s = s1` \\ fs []
+  \\ Cases_on `ns` \\ fs []
+  \\ metis_tac []);
+
+val SPLIT_IMP_Mem_NOT_IN = store_thm("SPLIT_IMP_Mem_NOT_IN",
+  ``SPLIT (st2heap p st) ({Mem y xs},c) ==>
+    !ys. ~(Mem y ys IN c)``,
+  fs [SPLIT_def] \\ rw [] \\ fs [EXTENSION,st2heap_def]
+  \\ CCONTR_TAC \\ fs []
+  \\ `Mem y ys ∈ store2heap st.refs` by metis_tac [Mem_NOT_IN_ffi2heap]
+  \\ `Mem y xs ∈ store2heap st.refs` by metis_tac [Mem_NOT_IN_ffi2heap]
+  \\ imp_res_tac store2heap_IN_unique_key \\ fs []);
+
+val FLOOKUP_FUPDATE_LIST = store_thm("FLOOKUP_FUPDATE_LIST",
+  ``!ns f. FLOOKUP (f |++ MAP (λn. (n,s)) ns) m =
+           if MEM m ns then SOME s else FLOOKUP f m``,
+  Induct \\ fs [FUPDATE_LIST] \\ rw [] \\ fs []
+  \\ fs [FLOOKUP_DEF,FAPPLY_FUPDATE_THM]);
+
+val ALL_DISTINCT_FLAT_MEM_IMP = store_thm("ALL_DISTINCT_FLAT_MEM_IMP",
+  ``!p2. ALL_DISTINCT (FLAT p2) /\ MEM ns' p2 /\ MEM ns p2 /\
+         MEM m ns' /\ MEM m ns ==> ns = ns'``,
+  Induct \\ fs [ALL_DISTINCT_APPEND] \\ rw [] \\ fs []
+  \\ res_tac \\ fs [MEM_FLAT] \\ metis_tac []);
+
+val ALL_DISTINCT_FLAT_FST_IMP = store_thm("ALL_DISTINCT_FLAT_FST_IMP",
+  ``!p2. ALL_DISTINCT (FLAT (MAP FST p2)) /\
+         MEM (ns,u') p2 /\ MEM (ns,u) p2 /\ ns <> [] ==> u = u'``,
+  Induct \\ fs [ALL_DISTINCT_APPEND] \\ rw [] \\ fs []
+  \\ fs [MEM_FLAT,MEM_MAP,FORALL_PROD]
+  \\ Cases_on `ns` \\ fs []
+  \\ first_x_assum (qspec_then `h` mp_tac) \\ fs []
+  \\ disch_then (qspec_then `h::t` mp_tac) \\ fs []
+  \\ rw [] \\ fs []);
+
+(*------------------------------------------------------------------*)
 (* Definition of the [cf] functions, that generates the characteristic
    formula of a cakeml expression *)
 
@@ -1096,13 +1327,6 @@ val cf_match_def = Define `
       exp2v env e = SOME v /\
       build_cases v rows env H Q)`
 
-val normalise_def = Define `
-  normalise x = (x:exp)` (* TODO: actually implement this without going into closures *)
-
-val evaluate_normalise = store_thm("evaluate_normalise",
-  ``evaluate F env s (normalise exp) res = evaluate F env s exp res``,
-  fs [normalise_def]);
-
 val cf_def = tDefine "cf" `
   cf (p:'ffi ffi_proj) (Lit l) = cf_lit l /\
   cf (p:'ffi ffi_proj) (Con opt args) = cf_con opt args /\
@@ -1284,70 +1508,6 @@ val cf_local = store_thm ("cf_local",
   )
 )
 
-(* Soundness of cf *)
-
-val htriple_valid_def = Define `
-  htriple_valid (p:'ffi ffi_proj) e env H Q =
-    !st h_i h_k.
-      SPLIT (st2heap p st) (h_i, h_k) ==>
-      H h_i ==>
-      ?v st' h_f h_g.
-        SPLIT3 (st2heap p st') (h_f, h_k, h_g) /\
-        evaluate F env st e (st', Rval v) /\
-        Q v h_f`
-
-val sound_def = Define `
-  sound (p:'ffi ffi_proj) e R =
-    !env H Q.
-      R env H Q ==>
-      htriple_valid p e env H Q`
-
-val star_split = Q.prove (
-  `!H1 H2 H3 H4 h1 h2 h3 h4.
-     ((H1 * H2) (h1 UNION h2) ==> (H3 * H4) (h3 UNION h4)) ==>
-     DISJOINT h1 h2 ==> H1 h1 ==> H2 h2 ==>
-     ?u v. H3 u /\ H4 v /\ SPLIT (h3 UNION h4) (u, v)`,
-  fs [STAR_def] \\ rpt strip_tac \\
-  `SPLIT (h1 UNION h2) (h1, h2)` by SPLIT_TAC \\
-  metis_tac []
-)
-
-val htriple_valid_normalise = store_thm ("htriple_valid_normalise",
-  ``!e env H Q.
-      htriple_valid (p:'ffi ffi_proj) (normalise e) env H Q <=>
-      htriple_valid (p:'ffi ffi_proj) e env H Q``,
-  fs [htriple_valid_def, evaluate_normalise]
-);
-
-val sound_local = store_thm ("sound_local",
-  ``!e R. sound (p:'ffi ffi_proj) e R ==> sound (p:'ffi ffi_proj) e (\env. local (R env))``,
-  rpt strip_tac \\ rewrite_tac [sound_def, htriple_valid_def] \\
-  fs [local_def] \\ rpt strip_tac \\
-  res_tac \\ rename1 `(H_i * H_k) h_i` \\ rename1 `R env H_i Q_f` \\
-  rename1 `SEP_IMPPOST (Q_f *+ H_k) (Q *+ H_g)` \\
-  fs [STAR_def] \\ rename1 `H_i h'_i` \\ rename1 `H_k h'_k` \\
-  `SPLIT (st2heap (p:'ffi ffi_proj) st) (h'_i, h_k UNION h'_k)` by SPLIT_TAC \\
-  qpat_x_assum `sound _ _ _` (progress o REWRITE_RULE [sound_def, htriple_valid_def]) \\
-  rename1 `SPLIT3 _ (h'_f, _, h'_g)` \\
-  fs [SEP_IMPPOST_def, STARPOST_def, SEP_IMP_def, STAR_def] \\
-  first_x_assum (qspecl_then [`v`, `h'_f UNION h'_k`] assume_tac) \\
-  `DISJOINT h'_f h'_k` by SPLIT_TAC \\
-  `?h_f h''_g. Q v h_f /\ H_g h''_g /\ SPLIT (h'_f UNION h'_k) (h_f, h''_g)` by
-    metis_tac [star_split] \\
-  Q.LIST_EXISTS_TAC [`v`, `st'`, `h_f`, `h'_g UNION h''_g`] \\ fs [] \\
-  SPLIT_TAC
-)
-
-val sound_false = store_thm ("sound_false",
-  ``!e. sound (p:'ffi ffi_proj) e (\env H Q. F)``,
-  rewrite_tac [sound_def]
-)
-
-val sound_local_false = Q.prove (
-  `!e. sound (p:'ffi ffi_proj) e (\env. local (\H Q. F))`,
-  strip_tac \\ HO_MATCH_MP_TAC sound_local \\ fs [sound_false]
-)
-
 val cf_base_case_tac =
   HO_MATCH_MP_TAC sound_local \\ rewrite_tac [sound_def, htriple_valid_def] \\
   rpt strip_tac \\ fs [] \\ res_tac \\
@@ -1370,125 +1530,6 @@ fun cf_evaluate_list_tac [] = prove_tac [bigStepTheory.evaluate_rules]
     once_rewrite_tac [bigStepTheory.evaluate_cases] \\ fs [] \\
     qexists_tac st \\ strip_tac THENL [fs [exp2v_evaluate], all_tac] \\
     cf_evaluate_list_tac sts
-
-val app_basic_of_htriple_valid = Q.prove (
-  `!clos body x env v H Q.
-    do_opapp [clos; x] = SOME (env, body) ==>
-    htriple_valid (p:'ffi ffi_proj) body env H Q ==>
-    app_basic (p:'ffi ffi_proj) clos x H Q`,
-  fs [app_basic_def, htriple_valid_def] \\ rpt strip_tac \\
-  first_x_assum progress \\ instantiate \\ SPLIT_TAC
-)
-
-val app_of_htriple_valid = Q.prove (
-  `!ns xvs env body H Q.
-     ns <> [] ==>
-     LENGTH ns = LENGTH xvs ==>
-     htriple_valid (p:'ffi ffi_proj) body (extend_env ns xvs env) H Q ==>
-     app (p:'ffi ffi_proj) (naryClosure env ns body) xvs H Q`,
-
-  Induct \\ rpt strip_tac \\ fs [naryClosure_def, LENGTH_CONS] \\ rw [] \\
-  rename1 `extend_env (n::ns) (xv::xvs) _` \\ Cases_on `ns` \\
-  fs [LENGTH_NIL, LENGTH_CONS] \\ rw [] \\
-  rfs [extend_env_def, Once extend_env_v_def, naryFun_def, app_def]
-  THEN1 (irule app_basic_of_htriple_valid \\ fs [extend_env_v_def, do_opapp_def])
-  THEN1 (
-    rename1 `extend_env_v (n'::ns) (xv'::xvs) _` \\
-    fs [app_basic_def] \\ rpt strip_tac \\ fs [do_opapp_def] \\
-    fs [SEP_EXISTS, cond_def, STAR_def, PULL_EXISTS, SPLIT_emp2] \\
-    fs [naryFun_def, naryClosure_def, Once bigStepTheory.evaluate_cases] \\
-    first_assum progress \\ instantiate \\ qexists_tac `{}` \\ SPLIT_TAC
-  )
-)
-
-val find_recfun_map = Q.prove (
-  `!l a b c f u v.
-     (!a b c. FST (f (a, b, c)) = a) ==>
-     f (a, b, c) = (a, u, v) ==>
-     find_recfun a l = SOME (b, c) ==>
-     find_recfun a (MAP f l) = SOME (u, v)`,
-  Induct_on `l`
-  THEN1 (fs [find_recfun_def]) \\ rpt gen_tac \\
-  NTAC 2 DISCH_TAC \\
-  rename1 `x::_` \\ PairCases_on `x` \\ rename1 `(a',b',c')` \\
-  rewrite_tac [Once find_recfun_def] \\ fs [] \\
-  Cases_on `a' = a` \\ fs [] \\ rpt strip_tac
-  THEN1 (fs [Once find_recfun_def])
-  THEN1 (
-    rewrite_tac [Once find_recfun_def] \\ fs [] \\
-    `?u' v'. f (a', b', c') = (a', u', v')` by (
-      first_assum (qspecl_then [`a'`, `b'`, `c'`] assume_tac) \\
-      qabbrev_tac `x' = f (a',b',c')` \\ PairCases_on `x'` \\ fs []
-    ) \\ fs [] \\
-    fs [Once find_recfun_def]
-  )
-)
-
-val app_rec_of_htriple_valid_aux = Q.prove (
-  `!f body params xvs funs naryfuns env H Q fvs.
-     params <> [] ==>
-     LENGTH params = LENGTH xvs ==>
-     naryfuns = letrec_pull_params funs ==>
-     ALL_DISTINCT (MAP (\ (f,_,_). f) naryfuns) ==>
-     find_recfun f naryfuns = SOME (params, body) ==>
-     htriple_valid (p:'ffi ffi_proj) body
-       (extend_env_rec (MAP (\ (f,_,_). f) naryfuns) fvs params xvs env)
-       H Q ==>
-     fvs = MAP (\ (f,_,_). naryRecclosure env naryfuns f) naryfuns ==>
-     app (p:'ffi ffi_proj) (naryRecclosure env naryfuns f) xvs H Q`,
-
-  Cases_on `params` \\ rpt strip_tac \\ rw [] \\
-  fs [LENGTH_CONS] \\ rfs [] \\ qpat_x_assum `xvs = _` (K all_tac) \\
-  rename1 `extend_env_rec _ _ (n::params) (xv::xvs) _` \\
-  Cases_on `params` \\ rfs [LENGTH_NIL, LENGTH_CONS] \\
-  fs [extend_env_rec_def, extend_env_v_rec_def] \\
-  fs [extend_env_def, extend_env_v_def, app_def]
-  THEN1 (
-    irule app_basic_of_htriple_valid \\
-    progress_then (fs o sing) do_opapp_naryRecclosure \\
-    fs [naryFun_def, letrec_pull_params_names, build_rec_env_zip]
-  )
-  THEN1 (
-    rw [] \\ rename1 `extend_env_v (n'::params) (xv'::xvs) _` \\
-    fs [app_basic_def] \\ rpt strip_tac \\
-    progress_then (fs o sing) do_opapp_naryRecclosure \\
-    fs [SEP_EXISTS, cond_def, STAR_def, PULL_EXISTS, SPLIT_emp2] \\
-    rename1 `SPLIT _ (h, i)` \\
-    `SPLIT3 (st2heap (p:'ffi ffi_proj) st) (h, {}, i)` by SPLIT_TAC \\
-    instantiate \\
-    (* fixme *)
-    qexists_tac `naryClosure
-      (env with v := (n,xv)::(ZIP (MAP (\ (f,_,_). f) (letrec_pull_params funs),
-        MAP (\ (f,_,_). naryRecclosure env (letrec_pull_params funs) f)
-            (letrec_pull_params funs)) ++ env.v))
-      (n'::params) body` \\ strip_tac
-    THEN1 (irule app_of_htriple_valid \\ fs [extend_env_def])
-    THEN1 (
-      fs [naryFun_def, naryClosure_def, Once bigStepTheory.evaluate_cases] \\
-      fs [letrec_pull_params_cancel, letrec_pull_params_names] \\
-      fs [build_rec_env_zip]
-    )
-  )
-)
-
-val app_rec_of_htriple_valid = Q.prove (
-  `!f params body funs xvs env H Q.
-     params <> [] ==>
-     LENGTH params = LENGTH xvs ==>
-     ALL_DISTINCT (MAP (\ (f,_,_). f) funs) ==>
-     find_recfun f (letrec_pull_params funs) = SOME (params, body) ==>
-     htriple_valid (p:'ffi ffi_proj) body
-       (extend_env_rec
-          (MAP (\ (f,_,_). f) funs)
-          (MAP (\ (f,_,_). naryRecclosure env (letrec_pull_params funs) f) funs)
-          params xvs env)
-        H Q ==>
-     app (p:'ffi ffi_proj) (naryRecclosure env (letrec_pull_params funs) f) xvs H Q`,
-  rpt strip_tac \\ irule app_rec_of_htriple_valid_aux
-  THEN1 (fs [letrec_pull_params_names])
-  THEN1 (qexists_tac `funs` \\ fs [])
-  THEN1 (instantiate \\ fs [letrec_pull_params_names])
-)
 
 val DROP_EL_CONS = Q.prove (
   `!l n.
@@ -1678,64 +1719,129 @@ val build_cases_evaluate_match = Q.prove (
   )
 )
 
-val SPLIT_SING_2 = store_thm("SPLIT_SING_2",
-  ``SPLIT s (x,{y}) <=> (s = y INSERT x) /\ ~(y IN x)``,
-  SPLIT_TAC);
-
-val sound_normalise = store_thm("sound_normalise",
-  ``sound p (normalise e) R <=> sound p e R``,
-  fs [sound_def, htriple_valid_normalise]);
-
-val SUBSET_IN = prove(
-  ``!s t x. s SUBSET t /\ x IN s ==> x IN t``,
-  fs [SUBSET_DEF] \\ metis_tac []);
-
-val SPLIT_FFI_SET_IMP_DISJOINT = store_thm("SPLIT_FFI_SET_IMP_DISJOINT",
-  ``SPLIT (st2heap p st) (c,{FFI_part s u ns}) ==>
-    !s1. ~(FFI_part s1 u ns IN c)``,
-  fs [SPLIT_def] \\ rw [] \\ fs [EXTENSION,st2heap_def,DISJOINT_DEF]
-  \\ CCONTR_TAC \\ fs []
-  \\ `FFI_part s1 u ns IN ffi2heap p st.ffi /\
-      FFI_part s u ns IN ffi2heap p st.ffi` by
-          metis_tac [FFI_part_NOT_IN_store2heap]
-  \\ PairCases_on `p`
-  \\ fs [ffi2heap_def]
-  \\ pop_assum mp_tac \\ IF_CASES_TAC \\ fs []
-  \\ CCONTR_TAC \\ fs []
-  \\ Cases_on `s = s1` \\ fs []
-  \\ Cases_on `ns` \\ fs []
-  \\ metis_tac []);
-
-val SPLIT_IMP_Mem_NOT_IN = store_thm("SPLIT_IMP_Mem_NOT_IN",
-  ``SPLIT (st2heap p st) ({Mem y xs},c) ==>
-    !ys. ~(Mem y ys IN c)``,
-  fs [SPLIT_def] \\ rw [] \\ fs [EXTENSION,st2heap_def]
-  \\ CCONTR_TAC \\ fs []
-  \\ `Mem y ys ∈ store2heap st.refs` by metis_tac [Mem_NOT_IN_ffi2heap]
-  \\ `Mem y xs ∈ store2heap st.refs` by metis_tac [Mem_NOT_IN_ffi2heap]
-  \\ imp_res_tac store2heap_IN_unique_key \\ fs []);
-
-val FLOOKUP_FUPDATE_LIST = store_thm("FLOOKUP_FUPDATE_LIST",
-  ``!ns f. FLOOKUP (f |++ MAP (λn. (n,s)) ns) m =
-           if MEM m ns then SOME s else FLOOKUP f m``,
-  Induct \\ fs [FUPDATE_LIST] \\ rw [] \\ fs []
-  \\ fs [FLOOKUP_DEF,FAPPLY_FUPDATE_THM]);
-
-val ALL_DISTINCT_FLAT_MEM_IMP = store_thm("ALL_DISTINCT_FLAT_MEM_IMP",
-  ``!p2. ALL_DISTINCT (FLAT p2) /\ MEM ns' p2 /\ MEM ns p2 /\
-         MEM m ns' /\ MEM m ns ==> ns = ns'``,
-  Induct \\ fs [ALL_DISTINCT_APPEND] \\ rw [] \\ fs []
-  \\ res_tac \\ fs [MEM_FLAT] \\ metis_tac []);
-
-val ALL_DISTINCT_FLAT_FST_IMP = store_thm("ALL_DISTINCT_FLAT_FST_IMP",
-  ``!p2. ALL_DISTINCT (FLAT (MAP FST p2)) /\
-         MEM (ns,u') p2 /\ MEM (ns,u) p2 /\ ns <> [] ==> u = u'``,
-  Induct \\ fs [ALL_DISTINCT_APPEND] \\ rw [] \\ fs []
-  \\ fs [MEM_FLAT,MEM_MAP,FORALL_PROD]
-  \\ Cases_on `ns` \\ fs []
-  \\ first_x_assum (qspec_then `h` mp_tac) \\ fs []
-  \\ disch_then (qspec_then `h::t` mp_tac) \\ fs []
-  \\ rw [] \\ fs []);
+val cf_ffi_sound = Q.prove (
+  `sound p (App (FFI ffi_index) [r]) (\env. local (\H Q.
+     ?rv. exp2v env r = SOME rv /\
+          app_ffi ffi_index rv H Q))`,
+   cf_strip_sound_tac \\
+   cf_evaluate_step_tac \\
+   `evaluate_list F env st [r] (st, Rval [rv])` by
+     (cf_evaluate_list_tac [`st`]) \\ instantiate \\
+   fs [do_app_def,app_ffi_def,SEP_IMP_def,W8ARRAY_def,SEP_EXISTS] \\
+   fs [STAR_def,cell_def,one_def,cond_def] \\
+   first_assum progress \\ fs [SPLIT_emp1] \\ rveq \\
+   fs [SPLIT_SING_2] \\ rveq \\
+   rename1 `F' u2` \\
+   `store_lookup y st.refs = SOME (W8array ws) /\
+    Mem y (W8array ws) IN st2heap p st` by
+     (`Mem y (W8array ws) IN st2heap p st` by SPLIT_TAC
+      \\ fs [st2heap_def,Mem_NOT_IN_ffi2heap]
+      \\ imp_res_tac store2heap_IN_EL
+      \\ imp_res_tac store2heap_IN_LENGTH
+      \\ fs [store_lookup_def] \\ NO_TAC) \\
+   fs [ffiTheory.call_FFI_def] \\
+   fs [IO_def,one_def] \\ rveq \\
+   fs [st2heap_def,FFI_part_NOT_IN_store2heap,Mem_NOT_IN_ffi2heap] \\
+   fs [SPLIT_SING_2] \\ rveq \\
+   `FFI_part s u ns IN store2heap st.refs ∪ ffi2heap p st.ffi` by SPLIT_TAC \\
+   fs [FFI_part_NOT_IN_store2heap] \\
+   pop_assum mp_tac \\
+   PairCases_on `p` \\
+   simp [Once ffi2heap_def] \\
+   IF_CASES_TAC \\ fs [] \\ strip_tac \\
+   first_assum drule \\ simp_tac std_ss [FLOOKUP_DEF] \\
+   rpt strip_tac \\ rveq \\
+   qpat_x_assum `parts_ok st.ffi (p0,p1)`
+         (fn th => mp_tac th \\ assume_tac th) \\
+   simp_tac std_ss [parts_ok_def] \\ strip_tac \\
+   qpat_x_assum `!x. _ ==> _` kall_tac \\
+   first_x_assum progress \\ fs [store_assign_def] \\
+   imp_res_tac store2heap_IN_EL \\
+   imp_res_tac store2heap_IN_LENGTH \\ fs [] \\
+   fs [store_v_same_type_def,PULL_EXISTS] \\ rveq \\
+   progress store2heap_LUPDATE \\ fs [] \\
+   fs [FLOOKUP_DEF] \\ rveq \\
+   first_assum progress \\ fs [] \\
+   qexists_tac `
+      (FFI_part s' u ns INSERT
+       (Mem y (W8array vs) INSERT u2))` \\
+   qexists_tac `{}` \\
+   `SPLIT (store2heap st.refs UNION ffi2heap (p0,p1) st.ffi)
+    (Mem y (W8array ws) INSERT u2 UNION h_k,
+     {FFI_part (p0 st.ffi.ffi_state ' ffi_index) u ns}) /\
+     SPLIT (store2heap st.refs UNION ffi2heap (p0,p1) st.ffi)
+     (Mem y (W8array ws) INSERT {},
+      u2 UNION h_k UNION
+      {FFI_part (p0 st.ffi.ffi_state ' ffi_index) u ns})` by SPLIT_TAC \\
+   fs [GSYM st2heap_def] \\
+   drule SPLIT_FFI_SET_IMP_DISJOINT \\
+   drule SPLIT_IMP_Mem_NOT_IN \\
+   ntac 2 strip_tac \\
+   reverse conj_tac THEN1
+    (first_assum match_mp_tac \\ fs [PULL_EXISTS,SPLIT_SING_2]) \\
+   match_mp_tac SPLIT3_of_SPLIT_emp3 \\
+   qpat_abbrev_tac `f1 = ffi2heap (p0,p1) _` \\
+   `f1 = (ffi2heap (p0,p1) st.ffi DELETE
+          FFI_part (p0 st.ffi.ffi_state ' ffi_index) u ns)
+         UNION {FFI_part s' u ns}` by all_tac THEN1
+     (unabbrev_all_tac \\ fs [ffi2heap_def] \\
+      reverse IF_CASES_TAC THEN1
+       (`F` by all_tac \\ pop_assum mp_tac \\ fs [] \\
+        fs [parts_ok_def] \\ metis_tac []) \\
+      fs [EXTENSION] \\ reverse (rw [] \\ EQ_TAC \\ rw [])
+      THEN1
+       (qpat_x_assum `_ = p0 y'` (fn th => fs [GSYM th]) \\
+        fs [FLOOKUP_FUPDATE_LIST])
+      THEN1
+       (qpat_x_assum `_ = p0 y'` (fn th => fs [GSYM th])
+        \\ Cases_on `MEM n ns` \\ fs [FLOOKUP_FUPDATE_LIST]
+        \\ `MEM ns (MAP FST p1) /\ MEM ns' (MAP FST p1)` by
+               (fs [MEM_MAP,EXISTS_PROD] \\ metis_tac [])
+        \\ metis_tac [ALL_DISTINCT_FLAT_MEM_IMP])
+      THEN1
+       (`ns <> ns'` by metis_tac [ALL_DISTINCT_FLAT_FST_IMP]
+        \\ qpat_x_assum `_ = p0 y'` (fn th => fs [GSYM th])
+        \\ Cases_on `MEM n ns` \\ fs [FLOOKUP_FUPDATE_LIST]
+        \\ `MEM ns (MAP FST p1) /\ MEM ns' (MAP FST p1)` by
+               (fs [MEM_MAP,EXISTS_PROD] \\ metis_tac [])
+        \\ metis_tac [ALL_DISTINCT_FLAT_MEM_IMP])
+      THEN1
+       (qpat_x_assum `_ = p0 y'` (fn th => fs [GSYM th])
+        \\ rpt strip_tac
+        \\ Cases_on `MEM n ns` \\ fs [FLOOKUP_FUPDATE_LIST]
+        \\ `MEM ns (MAP FST p1) /\ MEM ns' (MAP FST p1)` by
+               (fs [MEM_MAP,EXISTS_PROD] \\ metis_tac [])
+        \\ progress (ALL_DISTINCT_FLAT_MEM_IMP |> Q.INST [`m`|->`n`])
+        \\ rveq \\ fs [] \\ res_tac \\ fs [FLOOKUP_DEF])
+      \\ Cases_on `ns = ns'` \\ fs [] THEN1
+       (rveq  \\ first_x_assum drule
+        \\ qpat_x_assum `_ = p0 y'` (fn th => fs [GSYM th])
+        \\ fs [FLOOKUP_FUPDATE_LIST] \\ rw [] \\ disj2_tac
+        \\ metis_tac [ALL_DISTINCT_FLAT_FST_IMP])
+      \\ rw [] \\ first_assum drule
+      \\ qpat_x_assum `_ = p0 y'` (fn th => simp_tac std_ss [GSYM th])
+      \\ Cases_on `MEM n ns` \\ fs [FLOOKUP_FUPDATE_LIST]
+      \\ `MEM ns (MAP FST p1) /\ MEM ns' (MAP FST p1)` by
+             (fs [MEM_MAP,EXISTS_PROD] \\ metis_tac [])
+      \\ metis_tac [ALL_DISTINCT_FLAT_MEM_IMP]) \\
+   pop_assum (fn th => simp [th]) \\
+   pop_assum kall_tac \\
+   fs [st2heap_def] \\
+   simp [SPLIT_def] \\ reverse (rw [])
+   THEN1 SPLIT_TAC \\
+   fs [EXTENSION] \\ rw [] \\ EQ_TAC \\ rw [] \\ fs []
+   THEN1 SPLIT_TAC
+   THEN1 SPLIT_TAC
+   THEN1
+    (CCONTR_TAC \\ fs [] \\
+     `x = FFI_part (p0 st.ffi.ffi_state ' ffi_index) u ns` by SPLIT_TAC \\
+     Cases_on `x` \\ fs [] \\
+     fs [FFI_part_NOT_IN_store2heap])
+   \\ CCONTR_TAC \\ fs []
+   \\ `x IN u2 ∪ h_k ∪ {FFI_part (p0 st.ffi.ffi_state ' ffi_index) u ns} UNION {Mem y (W8array ws)}` by SPLIT_TAC
+   \\ pop_assum mp_tac
+   \\ fs [] \\ fs [ffi2heap_def] \\ rfs[]
+);
 
 val cf_sound = store_thm ("cf_sound",
   ``!p e. sound (p:'ffi ffi_proj) e (cf (p:'ffi ffi_proj) e)``,
@@ -1793,7 +1899,7 @@ val cf_sound = store_thm ("cf_sound",
     )
   )
   THEN1 (
-    (* Letrec *)
+    (* Letrec; the bulk of the proof is done in [cf_letrec_sound] *)
     HO_MATCH_MP_TAC sound_local \\ simp [MAP_MAP_o, o_DEF, LAMBDA_PROD] \\
     mp_tac (Q.SPECL [`funs`, `e`] cf_letrec_sound) \\
     fs [LAMBDA_PROD, letrec_pull_params_LENGTH, letrec_pull_params_names] \\
@@ -1805,127 +1911,12 @@ val cf_sound = store_thm ("cf_sound",
   )
   THEN1 (
     (* App *)
-    Cases_on `?ffi_index. op = FFI ffi_index` THEN1
-     (fs [] \\ rveq \\ TRY (MATCH_ACCEPT_TAC sound_local_false) \\
+    Cases_on `?ffi_index. op = FFI ffi_index` THEN1 (
+      (* FFI *)
+      fs [] \\ rveq \\
       (every_case_tac \\ TRY (MATCH_ACCEPT_TAC sound_local_false)) \\
-      cf_strip_sound_tac \\
-      cf_evaluate_step_tac \\
-      `evaluate_list F env st [h] (st, Rval [rv])` by
-        (cf_evaluate_list_tac [`st`]) \\ instantiate \\
-      fs [do_app_def,app_ffi_def,SEP_IMP_def,W8ARRAY_def,SEP_EXISTS] \\
-      fs [STAR_def,cell_def,one_def,cond_def] \\
-      first_assum progress \\ fs [SPLIT_emp1] \\ rveq \\
-      fs [SPLIT_SING_2] \\ rveq \\
-      rename1 `F' u2` \\
-      `store_lookup y st.refs = SOME (W8array ws) /\
-       Mem y (W8array ws) IN st2heap p st` by
-        (`Mem y (W8array ws) IN st2heap p st` by SPLIT_TAC
-         \\ fs [st2heap_def,Mem_NOT_IN_ffi2heap]
-         \\ imp_res_tac store2heap_IN_EL
-         \\ imp_res_tac store2heap_IN_LENGTH
-         \\ fs [store_lookup_def] \\ NO_TAC) \\
-      fs [ffiTheory.call_FFI_def] \\
-      fs [IO_def,one_def] \\ rveq \\
-      fs [st2heap_def,FFI_part_NOT_IN_store2heap,Mem_NOT_IN_ffi2heap] \\
-      fs [SPLIT_SING_2] \\ rveq \\
-      `FFI_part s u ns IN store2heap st.refs ∪ ffi2heap p st.ffi` by SPLIT_TAC \\
-      fs [FFI_part_NOT_IN_store2heap] \\
-      pop_assum mp_tac \\
-      PairCases_on `p` \\
-      simp [Once ffi2heap_def] \\
-      IF_CASES_TAC \\ fs [] \\ strip_tac \\
-      first_assum drule \\ simp_tac std_ss [FLOOKUP_DEF] \\
-      rpt strip_tac \\ rveq \\
-      qpat_x_assum `parts_ok st.ffi (p0,p1)`
-            (fn th => mp_tac th \\ assume_tac th) \\
-      simp_tac std_ss [parts_ok_def] \\ strip_tac \\
-      qpat_x_assum `!x. _ ==> _` kall_tac \\
-      first_x_assum progress \\ fs [store_assign_def] \\
-      imp_res_tac store2heap_IN_EL \\
-      imp_res_tac store2heap_IN_LENGTH \\ fs [] \\
-      fs [store_v_same_type_def,PULL_EXISTS] \\ rveq \\
-      progress store2heap_LUPDATE \\ fs [] \\
-      fs [FLOOKUP_DEF] \\ rveq \\
-      first_assum progress \\ fs [] \\
-      qexists_tac `
-         (FFI_part s' u ns INSERT
-          (Mem y (W8array vs) INSERT u2))` \\
-      qexists_tac `{}` \\
-      `SPLIT (store2heap st.refs UNION ffi2heap (p0,p1) st.ffi)
-       (Mem y (W8array ws) INSERT u2 UNION h_k,
-        {FFI_part (p0 st.ffi.ffi_state ' ffi_index) u ns}) /\
-        SPLIT (store2heap st.refs UNION ffi2heap (p0,p1) st.ffi)
-        (Mem y (W8array ws) INSERT {},
-         u2 UNION h_k UNION
-         {FFI_part (p0 st.ffi.ffi_state ' ffi_index) u ns})` by SPLIT_TAC \\
-      fs [GSYM st2heap_def] \\
-      drule SPLIT_FFI_SET_IMP_DISJOINT \\
-      drule SPLIT_IMP_Mem_NOT_IN \\
-      ntac 2 strip_tac \\
-      reverse conj_tac THEN1
-       (first_assum match_mp_tac \\ fs [PULL_EXISTS,SPLIT_SING_2]) \\
-      match_mp_tac SPLIT3_of_SPLIT_emp3 \\
-      qpat_abbrev_tac `f1 = ffi2heap (p0,p1) _` \\
-      `f1 = (ffi2heap (p0,p1) st.ffi DELETE
-             FFI_part (p0 st.ffi.ffi_state ' ffi_index) u ns)
-            UNION {FFI_part s' u ns}` by all_tac THEN1
-        (unabbrev_all_tac \\ fs [ffi2heap_def] \\
-         reverse IF_CASES_TAC THEN1
-          (`F` by all_tac \\ pop_assum mp_tac \\ fs [] \\
-           fs [parts_ok_def] \\ metis_tac []) \\
-         fs [EXTENSION] \\ reverse (rw [] \\ EQ_TAC \\ rw [])
-         THEN1
-          (qpat_x_assum `_ = p0 y'` (fn th => fs [GSYM th]) \\
-           fs [FLOOKUP_FUPDATE_LIST])
-         THEN1
-          (qpat_x_assum `_ = p0 y'` (fn th => fs [GSYM th])
-           \\ Cases_on `MEM n ns` \\ fs [FLOOKUP_FUPDATE_LIST]
-           \\ `MEM ns (MAP FST p1) /\ MEM ns' (MAP FST p1)` by
-                  (fs [MEM_MAP,EXISTS_PROD] \\ metis_tac [])
-           \\ metis_tac [ALL_DISTINCT_FLAT_MEM_IMP])
-         THEN1
-          (`ns <> ns'` by metis_tac [ALL_DISTINCT_FLAT_FST_IMP]
-           \\ qpat_x_assum `_ = p0 y'` (fn th => fs [GSYM th])
-           \\ Cases_on `MEM n ns` \\ fs [FLOOKUP_FUPDATE_LIST]
-           \\ `MEM ns (MAP FST p1) /\ MEM ns' (MAP FST p1)` by
-                  (fs [MEM_MAP,EXISTS_PROD] \\ metis_tac [])
-           \\ metis_tac [ALL_DISTINCT_FLAT_MEM_IMP])
-         THEN1
-          (qpat_x_assum `_ = p0 y'` (fn th => fs [GSYM th])
-           \\ rpt strip_tac
-           \\ Cases_on `MEM n ns` \\ fs [FLOOKUP_FUPDATE_LIST]
-           \\ `MEM ns (MAP FST p1) /\ MEM ns' (MAP FST p1)` by
-                  (fs [MEM_MAP,EXISTS_PROD] \\ metis_tac [])
-           \\ progress (ALL_DISTINCT_FLAT_MEM_IMP |> Q.INST [`m`|->`n`])
-           \\ rveq \\ fs [] \\ res_tac \\ fs [FLOOKUP_DEF])
-         \\ Cases_on `ns = ns'` \\ fs [] THEN1
-          (rveq  \\ first_x_assum drule
-           \\ qpat_x_assum `_ = p0 y'` (fn th => fs [GSYM th])
-           \\ fs [FLOOKUP_FUPDATE_LIST] \\ rw [] \\ disj2_tac
-           \\ metis_tac [ALL_DISTINCT_FLAT_FST_IMP])
-         \\ rw [] \\ first_assum drule
-         \\ qpat_x_assum `_ = p0 y'` (fn th => simp_tac std_ss [GSYM th])
-         \\ Cases_on `MEM n ns` \\ fs [FLOOKUP_FUPDATE_LIST]
-         \\ `MEM ns (MAP FST p1) /\ MEM ns' (MAP FST p1)` by
-                (fs [MEM_MAP,EXISTS_PROD] \\ metis_tac [])
-         \\ metis_tac [ALL_DISTINCT_FLAT_MEM_IMP]) \\
-      pop_assum (fn th => simp [th]) \\
-      pop_assum kall_tac \\
-      fs [st2heap_def] \\
-      simp [SPLIT_def] \\ reverse (rw [])
-      THEN1 SPLIT_TAC \\
-      fs [EXTENSION] \\ rw [] \\ EQ_TAC \\ rw [] \\ fs []
-      THEN1 SPLIT_TAC
-      THEN1 SPLIT_TAC
-      THEN1
-       (CCONTR_TAC \\ fs [] \\
-        `x = FFI_part (p0 st.ffi.ffi_state ' ffi_index) u ns` by SPLIT_TAC \\
-        Cases_on `x` \\ fs [] \\
-        fs [FFI_part_NOT_IN_store2heap])
-      \\ CCONTR_TAC \\ fs []
-      \\ `x IN u2 ∪ h_k ∪ {FFI_part (p0 st.ffi.ffi_state ' ffi_index) u ns} UNION {Mem y (W8array ws)}` by SPLIT_TAC
-      \\ pop_assum mp_tac
-      \\ fs [] \\ fs [ffi2heap_def] \\ rfs[]) \\
+      irule cf_ffi_sound
+    ) \\
     Cases_on `op` \\ fs [] \\ TRY (MATCH_ACCEPT_TAC sound_local_false) \\
     (every_case_tac \\ TRY (MATCH_ACCEPT_TAC sound_local_false)) \\
     cf_strip_sound_tac \\
@@ -2242,7 +2233,7 @@ val cf_sound = store_thm ("cf_sound",
     instantiate
   )
   THEN1 (
-    (* Mat *)
+    (* Mat: the bulk of the proof is done in [build_cases_evaluate_match] *)
     cf_strip_sound_full_tac \\
     `evaluate F env st e (st, Rval v)` by (fs [exp2v_evaluate]) \\
     instantiate \\ irule build_cases_evaluate_match \\
